---
title: Question-27
pagetitle: Question-27
order: 27
categories: [function]
---

For $\displaystyle x\in \mathbb{R}$, the function $\displaystyle f( x)$ satisfies the following identity:

$$
\begin{equation*}
2f( x) +f( 1-x) =x^{2}
\end{equation*}
$$

Find $\displaystyle f( 4)$.

::: {.callout-note title="Hint" collapse=true}

Substitute $x \rightarrow 1 - x$

:::

::: {.callout-note title="Answer" collapse=true}

$\cfrac{23}{3}$

:::

::: {.callout-note title="Solution" collapse=true}

Substituting $\displaystyle x\rightarrow 1-x$, we get:

$$
\begin{equation*}
2f( 1-x) +f( x) =( 1-x)^{2}
\end{equation*}
$$

Using this in conjunction with the original identity, we have:

$$
\begin{equation*}
2f( x) -\frac{f( x)}{2} =x^{2} -\frac{( 1-x)^{2}}{2}
\end{equation*}
$$

From this, we get:

$$
\begin{equation*}
f( x) =\frac{1}{3}\left[ x^{2} +2x-1\right]
\end{equation*}
$$

Plugging in $\displaystyle x=4$, we get $\displaystyle f( 4) =\frac{23}{3}$.

:::
